Desugaring scoped variables and partial proof
Desugaring scoped variables is achieved in two separate transformations.
First, the scoped variable names are made unique w.r.t. the entire program.
Second, the scoped variable names are removed.

This commit also contains a proof for the first transformation (making
scoped variables unique).

Other notable changes in this commit:

* WpShallow and ForallVarDeclsShallow are now opaque
* Rephrased ForallVarDeclsShallow and introduced lemmas to reason about it
* Added a lemma to test that scopes behave as expected for a concrete example

BoogieLang.dfy
@@ -1,9 +1,12 @@
 include "dafny-libraries/src/Wrappers.dfy"
 include "Util.dfy"
+include "dafny-libraries/src/Collections/Sequences/Seq.dfy"
 
 module BoogieLang {
   import opened Wrappers 
   import opened Util
+  import Sequences = Seq
+
 
   datatype Lit = LitInt(int) | LitBool(bool)
   {
@@ -57,7 +60,7 @@ module BoogieLang {
   type proc_name = string
   type lbl_name = string
   type tcon_name = string
-  type fun_name = string
+  type fun_name = string 
 
   datatype PrimTy = TBool | TInt
   {
@@ -88,6 +91,8 @@ module BoogieLang {
     case LitInt(_) => TInt
     case LitBool(_) => TBool
   }
+
+  type VarDecl = (var_name, Ty)
 
   datatype BinderKind = ForallQ | ExistsQ
   {
@@ -156,7 +161,7 @@ module BoogieLang {
     | Assert(Expr)
     | Assume(Expr)
     | Assign(var_name, Ty, Expr) 
-    | Havoc(seq<(var_name, Ty)>)
+    | Havoc(seq<VarDecl>)
     | SeqSimple(SimpleCmd, SimpleCmd) 
     /* The reason for adding a separate sequential composition for simple commands is to be able to transform the AST
        into a form that more directly represents the desired CFG block structure.
@@ -188,6 +193,17 @@ module BoogieLang {
         case SeqSimple(sc1, sc2) => return "TODO";
       }
     }
+
+    predicate WellFormedVars(xs: set<var_name>)
+    {
+      match this
+      case Skip => true
+      case Assert(e) => e.FreeVars() <= xs
+      case Assume(e) => e.FreeVars() <= xs
+      case Assign(x, t, e) => x in xs && e.FreeVars() <= xs
+      case Havoc(varDecls) => GetVarNames(varDecls) <= xs
+      case SeqSimple(sc1, sc2) => sc1.WellFormedVars(xs) && sc2.WellFormedVars(xs)
+    }
   }
 
 /** TODO: add return */
@@ -195,15 +211,35 @@ module BoogieLang {
     | SimpleCmd(SimpleCmd)
     | Break(Option<lbl_name>)
     | Seq(Cmd, Cmd)
-    | Scope(labelName: Option<lbl_name>, varDecls: seq<(var_name,Ty)>, body: Cmd)
+    | Scope(labelName: Option<lbl_name>, varDecls: seq<VarDecl>, body: Cmd)
     | Loop(invariants: seq<Expr>, body: Cmd) 
     //cond = None represents a non-deterministic if-statement (if(*) {...} else {...})
-    | If(Option<Expr>, thn: Cmd, els: Cmd)
+    | If(guard: Option<Expr>, thn: Cmd, els: Cmd)
   
   /*
     | ProcCall(proc_name, seq<Expr>, seq<var_name>)
   */
   {
+    predicate WellFormedVars(xs: set<var_name>)
+    {
+      match this
+      case SimpleCmd(sc) => sc.WellFormedVars(xs)
+      case Break(_) => true
+      case Scope(_, varDecls, body) =>
+        && Sequences.HasNoDuplicates(varDecls)
+        && body.WellFormedVars(xs+GetVarNames(varDecls))
+      case If(optCond, thn, els) =>
+        && (optCond.Some? ==> optCond.value.FreeVars() <= xs)
+        && thn.WellFormedVars(xs)
+        && els.WellFormedVars(xs)
+      case Loop(invs, body) =>
+        && (forall inv | inv in invs :: inv.FreeVars() <= xs)
+        && body.WellFormedVars(xs)
+      case Seq(c1, c2) =>
+        && c1.WellFormedVars(xs)
+        && c2.WellFormedVars(xs)
+    }
+
     method ToString(indent: nat) returns (s: string) {
       match this {
         case SimpleCmd(simpleC) => s := simpleC.ToString(indent); return s;
@@ -275,6 +311,11 @@ module BoogieLang {
     case AbsV(abs_val) => TCon(a(abs_val))
   }
 
+  function TypeOfValues<A>(a: absval_interp<A>, vs: seq<Val<A>>) : seq<Ty>
+  {
+    seq(|vs|, i requires 0 <= i < |vs| => TypeOfVal(a, vs[i]))
+  }
+
   type state<A> = map<var_name, Val<A>>
 
   //while loop without break in body
@@ -316,7 +357,23 @@ module BoogieLang {
 
   function method GetVarNames(vs: seq<(var_name,Ty)>):set<var_name>
   {
-    if |vs| == 0 then {} else {vs[0].0} + GetVarNames(vs[1..])
+    //if |vs| == 0 then {} else {vs[0].0} + GetVarNames(vs[1..])
+    set varDecl | varDecl in vs :: varDecl.0
+  }
+
+  function method GetVarNamesSeq(vs: seq<(var_name,Ty)>):seq<var_name>
+  {
+    seq(|vs|, i requires 0 <= i < |vs| => vs[i].0)
+  }
+
+  lemma GetVarNamesContainedSeq(v: var_name, vs: seq<(var_name,Ty)>)
+    requires v in GetVarNames(vs)  
+    ensures v in GetVarNamesSeq(vs)
+  {
+    var varDecl :| varDecl in vs && varDecl.0 == v;
+    var i :| 0 <= i < |vs| && varDecl == vs[i];
+
+    assert GetVarNamesSeq(vs)[i] == vs[i].0;
   }
 
   function ModifiedVars(c: Cmd): seq<(var_name, Ty)>
