DesugarScopedVarsImpl.dfy
@@ -1,0 +1,174 @@
+include "BoogieSemantics.dfy"
+include "dafny-libraries/src/Collections/Sequences/Seq.dfy"
+include "dafny-libraries/src/Collections/Maps/Maps.dfy"
+include "Naming.dfy"
+
+module DesugarScopedVarsImpl {
+
+  import opened BoogieLang
+  import opened BoogieSemantics
+  import Sequences = Seq
+  import Maps
+  import Util
+  import opened Wrappers
+  import opened Naming
+
+ function method MultiSubstExpr(e: Expr, varMapping: map<var_name, var_name>): Expr
+
+ lemma MultiSubstExprSpec<A(!new)>(a: absval_interp<A>, varMapping: map<var_name, var_name>, e: Expr, s1: state<A>, s2: state<A>)
+    requires forall x | x in e.FreeVars() :: 
+      && (x in varMapping.Keys ==> Maps.Get(s1, x) == Maps.Get(s2, varMapping[x]))
+      && (x !in varMapping.Keys ==> Maps.Get(s1, x) == Maps.Get(s2, x))
+    ensures EvalExpr(a, e, s1) == EvalExpr(a, MultiSubstExpr(e, varMapping), s2)
+  
+ lemma MultiSubstExprSpec2<A(!new)>(a: absval_interp<A>, varMapping: map<var_name, var_name>, e: Expr, s1: state<A>, s2: state<A>)
+    requires (forall k | k in varMapping.Keys :: Maps.Get(s1, k) == Maps.Get(s2, varMapping[k]))
+    requires e.FreeVars() <= varMapping.Keys
+    ensures EvalExpr(a, e, s1) == EvalExpr(a, MultiSubstExpr(e, varMapping), s2)
+  {
+    MultiSubstExprSpec(a, varMapping, e, s1, s2);
+  }
+
+  function method SubstSimpleCmd(sc: SimpleCmd, varMapping: map<var_name, var_name>) : SimpleCmd
+  {
+    match sc
+    case Skip => Skip 
+    case Assert(e) => Assert(MultiSubstExpr(e, varMapping))
+    case Assume(e) => Assume(MultiSubstExpr(e, varMapping))
+    case Assign(x, t, e) =>
+      var newLHS := if x in varMapping.Keys then varMapping[x] else x;
+      var newRHS := MultiSubstExpr(e, varMapping);
+      Assign(newLHS, t, newRHS)
+    case Havoc(varDecls) =>
+      var f := (vDecl : (var_name, Ty)) => 
+          if vDecl.0 in varMapping.Keys then (varMapping[vDecl.0], vDecl.1) else vDecl;
+      var varDecls' := Sequences.Map(f, varDecls);
+      Havoc(varDecls')
+    case SeqSimple(c1, c2)  =>
+      SeqSimple(SubstSimpleCmd(c1, varMapping), SubstSimpleCmd(c2, varMapping))
+  }
+
+  function method CreateUniqueVarDecls(varDecls: seq<(var_name, Ty)>, counter: nat) : seq<(var_name,Ty)>
+    ensures 
+      var varDecls' := CreateUniqueVarDecls(varDecls, counter);
+      && |varDecls'| == |varDecls|
+      && GetVarNames(varDecls') <= VarNameSet(GetVarNames(varDecls), counter, counter + |varDecls|)
+  {
+    /** TODO
+      Currently, a suffix is added to every variable even if there are no clashes. 
+      This makes it harder to read the target output. It would be nice if one could 
+      reuse a name if it does not clash with anything else that has been so far. 
+      Doing this would require a fold to avoid updating the counter if a name is 
+      reused. Such a change would require restructuring the proof of the transformation
+      making the names unique. 
+      Alternatively, one could apply such a transformation later to remove the counters
+      from names that don't require them. 
+     */
+    var res := seq(|varDecls|, i requires 0 <= i < |varDecls| => (VersionedName(varDecls[i].0, counter+i), varDecls[i].1));
+    assert GetVarNames(res) <= VarNameSet(GetVarNames(varDecls), counter, counter + |varDecls|) by {
+      /** we reveal VarNameSet() inside this by clause, because if it's done outside by clause, then
+          VarNameSet() is revealed to all callers of this function (this behaviour is a bug, see 
+          https://github.com/dafny-lang/dafny/issues/1382) 
+      */
+      reveal VarNameSet();
+    }
+    res
+  }
+
+  lemma CreateUniqueVarDeclsNoDup(varDecls: seq<(var_name, Ty)>, counter: nat)
+    ensures 
+      var varDecls' := CreateUniqueVarDecls(varDecls, counter);
+      Sequences.HasNoDuplicates(GetVarNamesSeq(varDecls'))
+  {
+    var varDecls' := CreateUniqueVarDecls(varDecls, counter);
+    var varNames' := GetVarNamesSeq(varDecls');
+    forall i, j | 0 <= i < |varNames'| && 0 <= j < |varNames'| && i != j
+    ensures varNames'[i] != varNames'[j]
+    {
+      calc {
+        varNames'[i];
+        VersionedName(varDecls[i].0, counter+i);
+      != { VersionedNameInjective(varDecls[i].0, varDecls[j].0, counter+i, counter+j); }
+        VersionedName(varDecls[j].0, counter+j);
+        varNames'[j];
+      }
+    }
+    reveal Sequences.HasNoDuplicates();
+  }
+
+  function method ConvertVDeclsToSubstMap(varDecls: seq<(var_name, Ty)>, varDecls': seq<(var_name, Ty)>) : map<var_name, var_name>
+    requires |varDecls| == |varDecls'|
+    ensures 
+      var res := ConvertVDeclsToSubstMap(varDecls, varDecls');
+      && res.Keys == GetVarNames(varDecls)
+      && res.Values <= GetVarNames(varDecls')
+  {
+    if |varDecls| == 0 then
+      map[]
+    else
+      var oldName:= varDecls[0].0;
+      var newName := varDecls'[0].0;
+      var m' := ConvertVDeclsToSubstMap(varDecls[1..], varDecls'[1..]);
+      var m := m'[oldName := newName];
+      assert m.Values <= {newName} + GetVarNames(varDecls'[1..]);
+      m
+  }
+
+  /*
+  * substMap: active variables that are mapped
+  * freshVars: all fresh variable declarations
+  */
+  function method MakeScopedVarsUnique(
+    c: Cmd, 
+    substMap: map<var_name, var_name>, 
+    counter: nat): (Cmd, nat)
+    ensures
+      var (_, counter') := MakeScopedVarsUnique(c, substMap, counter);
+      counter <= counter'
+  {
+    match c
+    case SimpleCmd(sc) => (SimpleCmd(SubstSimpleCmd(sc, substMap)), counter)
+    case Break(_) => (c, counter)
+    case Seq(c1, c2) => 
+      var (c1', counter1') := MakeScopedVarsUnique(c1, substMap, counter);
+      var (c2', counter2') := MakeScopedVarsUnique(c2, substMap, counter1');
+      (Seq(c1', c2'), counter2')
+    case Scope(optLabel, varDecls, body) =>
+      var varDecls' := CreateUniqueVarDecls(varDecls, counter);
+      var counter' := counter + |varDecls'|;
+      var substMap' := substMap + ConvertVDeclsToSubstMap(varDecls, varDecls');
+      var (body'', counter'') := MakeScopedVarsUnique(body, substMap', counter');
+      (Scope(optLabel, varDecls', body''), counter'')
+    case If(None, thn, els) => 
+      //TODO: make sure If(Some(...)) has been desugared
+      var (thn', counter') := MakeScopedVarsUnique(thn, substMap, counter);
+      var (els', counter'') := MakeScopedVarsUnique(els, substMap, counter');
+      (If(None, thn', els'), counter'')
+    case _ => (c, counter) //TODO (precondition should eliminate this case)
+  }  
+ 
+  function method RemoveScopedVars(c: Cmd): (Cmd, (seq<(var_name, Ty)>))
+    /*requires substMap.Values <= set c,x | x in substMap.Keys && 0 < c < usedVars.1 :: VersionedName(x, c)
+    requires forall x | x in substMap.Keys :: exists c : nat :: c <= usedVars.1 && substMap[x] == VersionedName(x, c)
+    ensures 
+      forall x | x in substMap.Keys :: exists c : nat :: c <= usedVars.1 && substMap[x] == VersionedName(x, c)*/
+  {
+    match c
+    case SimpleCmd(sc) => (c, [])
+    case Break(_) => (c, [])
+    case Seq(c1, c2) => 
+      var (c1', decls1) := RemoveScopedVars(c1);
+      var (c2', decls2) := RemoveScopedVars(c2);
+      (Seq(c1', c2'), decls1 + decls2)
+    case Scope(optLabel, varDecls, body) =>
+      var (body', declsBody) := RemoveScopedVars(body);
+      (Scope(optLabel, [], body'), varDecls + declsBody)
+    case If(None, thn, els) => 
+      //TODO: make sure If(Some(...)) has been desugared
+      var (thn', declsThn) := RemoveScopedVars(thn);
+      var (els', declsEls) := RemoveScopedVars(els);
+      (If(None, thn', els'), declsThn + declsEls)
+    case _ => (c, []) //TODO (precondition should eliminate this case)
+  }
+
+}
