MakeScopedVarsUniqueProof.dfy
@@ -1,0 +1,909 @@
+include "BoogieSemantics.dfy"
+include "DesugarScopedVarsImpl.dfy"
+include "Naming.dfy"
+include "dafny-libraries/src/Collections/Sequences/Seq.dfy"
+include "dafny-libraries/src/Collections/Maps/Maps.dfy"
+
+module MakeScopedVarsUniqueProof {
+
+  import opened BoogieLang
+  import opened BoogieSemantics
+  import Sequences = Seq
+  import Maps
+  import Util
+  import opened Wrappers
+  import opened DesugarScopedVarsImpl
+  import opened Naming
+
+  type MapOrig<V> = map<var_name, Option<V>>
+
+  lemma UnionOfInjectiveMaps<K,V>(m1: map<K,V>, m2: map<K,V>)
+    requires 
+      && Maps.Injective(m1)
+      && Maps.Injective(m2)
+      && m1.Values !! m2.Values
+    ensures Maps.Injective(m1 + m2)
+  {
+    var m := m1 + m2;
+    reveal Maps.Injective();
+
+    forall x, x' | x != x' && x in m && x' in m
+    ensures m[x] != m[x']
+    {
+      if x in m2.Keys && x' in m2.Keys {
+        // conclusion follows from Maps.Injective(m1)
+      } else if x !in m2.Keys && x' !in m2.Keys {
+        // conclusion follows from Maps.Injective(m2)
+      } else {
+        var y1 := if x in m2.Keys then x' else x;
+        var y2 := if x in m2.Keys then x else x';
+
+        assert m[y1] != m[y2] by {
+          assert m[y1] == m1[y1];
+          assert m[y2] == m2[y2];
+          assert m1[y1] in m1.Values;
+          assert m2[y2] in m2.Values;
+        }
+      }
+    }
+  }
+
+  predicate {:opaque} RelState<V>(m: map<var_name, var_name>, s1: map<var_name, V>, s2: map<var_name, V>, s2Orig: map<var_name, Option<V>>)
+  {
+    && (forall k | k in m.Keys :: Maps.Get(s1, k) == Maps.Get(s2, m[k]))
+    && (forall k | k in s2Orig.Keys :: Maps.Get(s2, k) == s2Orig[k])
+    && m.Values !! s2Orig.Keys
+  }
+
+  predicate {:opaque} RelPred<A(!new)>(m: map<var_name, var_name>, post1: Predicate<A>, post2: Predicate<A>, s2Orig: MapOrig<Val<A>>)
+  {
+    forall s, s' | RelState(m, s, s', s2Orig) :: post1(s) == post2(s')
+  }
+
+  lemma RelStateUpdPreserve<V>(varMapping: map<var_name, var_name>, s1: map<var_name, V>, s2: map<var_name, V>, s2Orig: MapOrig<V>, x: var_name, v: V)
+  requires RelState(varMapping, s1, s2, s2Orig)
+  requires Maps.Injective(varMapping)
+  requires x in varMapping.Keys
+  ensures RelState(varMapping, s1[x := v], s2[varMapping[x] := v], s2Orig)
+  {
+    reveal RelState();
+    var x' := varMapping[x];
+    forall k | k in varMapping.Keys 
+    ensures Maps.Get(s1[x := v], k) == Maps.Get(s2[varMapping[x] := v], varMapping[k])
+    {
+      var k' := varMapping[k];
+      if k != x {
+        calc {
+          Maps.Get(s1[x := v], k);
+          Maps.Get(s1, k);
+          Maps.Get(s2, k');
+          { reveal Maps.Injective(); }
+          Maps.Get(s2[x' := v], k');
+        }
+      }
+    }
+  }
+
+  lemma RelStateUpdVarDeclsPreserve<A>(
+      varMapping: map<var_name, var_name>, 
+      s1: state<A>,
+      s2: state<A>, 
+      s2Orig: MapOrig<Val<A>>, 
+      varDecls: seq<VarDecl>, 
+      varDecls': seq<VarDecl>,
+      vs: seq<Val<A>>)
+  requires RelState(varMapping, s1, s2, s2Orig)
+  requires Maps.Injective(varMapping)
+  requires GetVarNames(varDecls) <= varMapping.Keys
+  requires |vs| == |varDecls| == |varDecls'|
+  requires (forall i | 0 <= i < |varDecls| :: varDecls'[i].0 == varMapping[varDecls[i].0])
+  ensures RelState(varMapping, StateUpdVarDecls(s1, varDecls, vs), StateUpdVarDecls(s2, varDecls', vs), s2Orig)
+  {
+    if |varDecls| > 0 {       
+        var s1' := StateUpdVarDecls(s1, varDecls[1..], vs[1..]);
+        var s2' := StateUpdVarDecls(s2, varDecls'[1..], vs[1..]);
+
+        assert RelState(varMapping, s1', s2', s2Orig) by {
+          RelStateUpdVarDeclsPreserve(varMapping, s1, s2, s2Orig, varDecls[1..], varDecls'[1..], vs[1..]);
+        }
+
+        RelStateUpdPreserve(varMapping, s1', s2', s2Orig, varDecls[0].0, vs[0]);
+    }
+  }
+
+  lemma ForallVarDeclRel<A(!new)>(
+      a: absval_interp<A>, 
+      varDecls: seq<(var_name, Ty)>, 
+      varMapping: map<var_name, var_name>, 
+      p1: Predicate<A>,
+      p2: Predicate<A>,
+      s2Orig: MapOrig<Val<A>>)
+      requires RelPred(varMapping, p1, p2, s2Orig)
+      requires GetVarNames(varDecls) <= varMapping.Keys
+      requires Maps.Injective(varMapping)
+      ensures 
+        var f := (vDecl : (var_name, Ty)) => 
+            if vDecl.0 in varMapping.Keys then (varMapping[vDecl.0], vDecl.1) else vDecl;
+        var varDecls' := Sequences.Map(f, varDecls);
+        RelPred(varMapping, ForallVarDeclsShallow(a, varDecls, p1), ForallVarDeclsShallow(a, varDecls', p2), s2Orig)
+    {
+      var f := (vDecl : (var_name, Ty)) => 
+          if vDecl.0 in varMapping.Keys then (varMapping[vDecl.0], vDecl.1) else vDecl;
+      var varDecls' := Sequences.Map(f, varDecls);
+      if |varDecls| == 0 {
+        //trivial
+        reveal ForallVarDeclsShallow();
+        assert ForallVarDeclsShallow(a, varDecls, p1) == p1;
+      } else {
+        var (x,t) := varDecls[0];
+        var x' := varMapping[x];
+
+        var f := (vDecl : (var_name, Ty)) => 
+            if vDecl.0 in varMapping.Keys then (varMapping[vDecl.0], vDecl.1) else vDecl;
+        var varDecls' := Sequences.Map(f, varDecls);
+
+        forall s1, s2 | RelState(varMapping, s1, s2, s2Orig)
+        ensures ForallVarDeclsShallow(a, varDecls, p1)(s1) == ForallVarDeclsShallow(a, varDecls', p2)(s2)
+        {
+          forall vs | ValuesRespectDecls(a, vs, varDecls)
+          ensures p1(StateUpdVarDecls(s1, varDecls, vs)) == p2(StateUpdVarDecls(s2, varDecls', vs))
+          {
+            var s1' := StateUpdVarDecls(s1, varDecls, vs);
+            var s2' := StateUpdVarDecls(s2, varDecls', vs);
+            assert RelState(varMapping, s1', s2', s2Orig) by {
+              RelStateUpdVarDeclsPreserve(varMapping, s1, s2, s2Orig, varDecls, varDecls', vs);
+            }
+            reveal RelPred();
+          }
+          ForallVarDeclsShallowEquiv(a, varDecls, varDecls', p1, p2, s1, s2);
+        }
+
+        reveal RelPred();
+      }
+    }
+
+  lemma ForallVarDeclRel2<A(!new)>(
+      a: absval_interp<A>, 
+      varDecls: seq<(var_name, Ty)>, 
+      varMapping: map<var_name, var_name>, 
+      p1: Predicate<A>,
+      p2: Predicate<A>,
+      s1: state<A>,
+      s2: state<A>,
+      sOrig: MapOrig<Val<A>>)
+      requires RelPred(varMapping, p1, p2, sOrig)
+      requires RelState(varMapping, s1, s2, sOrig)
+      requires GetVarNames(varDecls) <= varMapping.Keys
+      requires Maps.Injective(varMapping)
+      ensures 
+        var f := (vDecl : (var_name, Ty)) => 
+            if vDecl.0 in varMapping.Keys then (varMapping[vDecl.0], vDecl.1) else vDecl;
+        var varDecls' := Sequences.Map(f, varDecls);
+        ForallVarDeclsShallow(a, varDecls, p1)(s1) ==  ForallVarDeclsShallow(a, varDecls', p2)(s2)
+    {
+      ForallVarDeclRel(a, varDecls, varMapping, p1, p2, sOrig);
+      reveal RelPred();
+    }
+
+  lemma {:induction false} SubstSimpleCmdCorrect<A(!new)>(a: absval_interp<A>, sc: SimpleCmd, varMapping: map<var_name, var_name>, 
+      post1: Predicate<A>, post2: Predicate<A>, s2Orig: MapOrig<Val<A>>)
+      requires RelPred(varMapping, post1, post2, s2Orig)
+      requires sc.WellFormedVars(varMapping.Keys)
+      requires Maps.Injective(varMapping)
+      ensures 
+        var sc' := SubstSimpleCmd(sc, varMapping);
+        RelPred(varMapping, WpShallowSimpleCmd(a, sc, post1), WpShallowSimpleCmd(a, sc', post2), s2Orig)
+    {
+      var sc' := SubstSimpleCmd(sc, varMapping);
+      var pre1 := WpShallowSimpleCmd(a, sc, post1);
+      var pre2 := WpShallowSimpleCmd(a, sc', post2);
+      forall s1:map<var_name, Val<A>>, s2 | RelState(varMapping, s1, s2, s2Orig)
+        ensures pre1(s1) == pre2(s2)
+      {
+        reveal RelPred();
+        match sc {
+          case Skip => 
+          case Assume(e) => 
+            reveal RelState();
+            MultiSubstExprSpec2(a, varMapping, e, s1, s2);
+          case Assert(e) => 
+            reveal RelState();
+            reveal RelPred();
+            MultiSubstExprSpec2(a, varMapping, e, s1, s2);
+          case Assign(x, t, e) =>
+            var e' := MultiSubstExpr(e, varMapping);
+            var v1Opt := EvalExpr(a, e, s1);
+            var v2Opt := EvalExpr(a, e', s2);
+            assert v1Opt == v2Opt by {
+              reveal RelState();
+              MultiSubstExprSpec2(a, varMapping, e, s1, s2);
+            }
+
+            if(v1Opt.Some?) {
+              var v := v1Opt.value;
+              var x' := varMapping[x];
+
+              assert RelState(varMapping, s1[x := v], s2[x' := v], s2Orig) by {
+                RelStateUpdPreserve(varMapping, s1, s2, s2Orig, x, v);
+              }
+            }
+          case Havoc(vDecls) => 
+            var f := 
+              (vDecl : (var_name, Ty)) => 
+                    if vDecl.0 in varMapping.Keys then (varMapping[vDecl.0], vDecl.1) else vDecl;
+            var vDecls' := Sequences.Map(f, vDecls);
+            
+            calc {
+              WpShallowSimpleCmd(a, Havoc(vDecls), post1)(s1);
+              ForallVarDeclsShallow(a, vDecls, post1)(s1);
+              { ForallVarDeclRel2(a, vDecls, varMapping, post1, post2, s1, s2, s2Orig); }
+              ForallVarDeclsShallow(a, vDecls', post2)(s2);
+              WpShallowSimpleCmd(a, Havoc(vDecls'), post2)(s2);
+              WpShallowSimpleCmd(a, SubstSimpleCmd(Havoc(vDecls), varMapping), post2)(s2);
+            }
+          case SeqSimple(sc1, sc2) =>
+            var sc1' := SubstSimpleCmd(sc1, varMapping);
+            var sc2' := SubstSimpleCmd(sc2, varMapping);
+
+            var post1' := WpShallowSimpleCmd(a, sc2, post1);
+            var post2' := WpShallowSimpleCmd(a, sc2', post2);
+
+
+            calc {
+              WpShallowSimpleCmd(a, SeqSimple(sc1, sc2), post1)(s1);
+              WpShallowSimpleCmd(a, sc1, post1')(s1);
+              { 
+                assert RelPred(varMapping, post1', post2', s2Orig) by {
+                  SubstSimpleCmdCorrect(a, sc2, varMapping, post1, post2, s2Orig);
+                }
+                SubstSimpleCmdCorrect(a, sc1, varMapping, post1', post2', s2Orig); 
+              }
+              WpShallowSimpleCmd(a, sc1', post2')(s2);
+              WpShallowSimpleCmd(a, SeqSimple(sc1', sc2'), post2)(s2);
+            }
+        }
+      }
+    }
+
+    predicate {:opaque} RelPost<A(!new)>(m: map<var_name, var_name>, post1: WpPostShallow<A>, post2: WpPostShallow<A>, s2Orig: MapOrig<Val<A>>)
+    {
+      && post1.scopes.Keys == post2.scopes.Keys
+      && RelPred(m, post1.normal, post2.normal, s2Orig)
+      && RelPred(m, post1.currentScope, post2.currentScope, s2Orig)
+      && (forall lbl | lbl in post1.scopes.Keys :: RelPred(m, post1.scopes[lbl], post2.scopes[lbl], s2Orig))
+    }
+
+    lemma ResetVarsStateLookup<A(!new)>(varDecls: seq<VarDecl>, s: state<A>, sOrig: state<A>, x: var_name)
+    requires x in GetVarNames(varDecls)
+    ensures Maps.Get(ResetVarsState(varDecls, s, sOrig), x) == Maps.Get(sOrig, x)
+    { }
+
+    lemma ResetVarsStateLookup2<A(!new)>(varDecls: seq<VarDecl>, s: state<A>, sOrig: state<A>, x: var_name)
+    requires x !in GetVarNames(varDecls)
+    ensures Maps.Get(ResetVarsState(varDecls, s, sOrig), x) == Maps.Get(s, x)
+    { }
+
+    lemma RelStateSwitch<A(!new)>(
+      m: map<var_name, var_name>, 
+      varDecls: seq<VarDecl>, 
+      varDecls': seq<VarDecl>,
+      sA: state<A>, 
+      sB: state<A>, 
+      s1: state<A>,
+      s2: state<A>,
+      s2Orig: MapOrig<Val<A>>)
+    requires |varDecls| == |varDecls'|
+    requires m.Values !! GetVarNames(varDecls')
+    requires s2Orig.Keys !! GetVarNames(varDecls')
+    requires 
+      var s2OrigNewKeys := set x | x in GetVarNames(varDecls) && x in m.Keys :: m[x];
+      var s2Orig' := s2Orig + map x' | x' in s2OrigNewKeys :: Maps.Get(s2, x');
+      var m' := m + ConvertVDeclsToSubstMap(varDecls, varDecls');
+      && RelState(m', sA, sB, s2Orig')
+      && RelState(m, s1, s2, s2Orig)
+    requires |varDecls| == |varDecls'|
+    ensures 
+      RelState(m, ResetVarsState(varDecls, sA, s1), ResetVarsState(varDecls', sB, s2), s2Orig)
+    {
+      reveal RelState();
+
+      var s2OrigNewKeys := set x | x in GetVarNames(varDecls) && x in m.Keys :: m[x];
+      var s2Orig' := s2Orig + map x' | x' in s2OrigNewKeys :: Maps.Get(s2, x');
+      var mExt := ConvertVDeclsToSubstMap(varDecls, varDecls');
+      var m' := m + mExt;
+
+      var sA' := ResetVarsState(varDecls, sA, s1);
+      var sB' := ResetVarsState(varDecls', sB, s2);
+
+      forall k | k in m.Keys
+      ensures Maps.Get(sA', k) == Maps.Get(sB', m[k])
+      {
+        if k in mExt {
+          assert k in GetVarNames(varDecls);
+          assert m[k] in s2OrigNewKeys;
+          calc {
+            Maps.Get(sB', m[k]);
+            {
+              assert m[k] !in GetVarNames(varDecls');
+              ResetVarsStateLookup2(varDecls', sB, s2, m[k]);
+            }
+            Maps.Get(sB, m[k]);
+            s2Orig'[m[k]];
+            Maps.Get(s2, m[k]);
+            Maps.Get(s1, k);
+            {
+              ResetVarsStateLookup(varDecls, sA, s1, k);
+            }
+            Maps.Get(sA', k);
+          }
+        } else {
+          calc {
+            Maps.Get(sB', m[k]);
+            {
+              assert m[k] !in GetVarNames(varDecls');
+              ResetVarsStateLookup2(varDecls', sB, s2, m[k]);
+            }
+            Maps.Get(sB, m[k]);
+            Maps.Get(sA, k);
+            {
+              assert k !in GetVarNames(varDecls);
+              ResetVarsStateLookup2(varDecls, sA, s1, k);
+            }
+            Maps.Get(sA', k);
+          }
+        }
+      }
+
+      forall k | k in s2Orig.Keys
+      ensures Maps.Get(sB', k) == s2Orig[k]
+      {
+        assert m'.Values !! s2Orig'.Keys;
+        assert m.Values !! s2Orig.Keys;
+        assert m.Values !! GetVarNames(varDecls');
+
+        calc {
+          Maps.Get(sB', k);
+          {
+            assert k !in GetVarNames(varDecls');
+            ResetVarsStateLookup2(varDecls', sB, s2, k);
+          }
+          Maps.Get(sB, k);
+          s2Orig'[k];
+          s2Orig[k];
+        }
+      }
+    }
+
+  lemma RelPredSwitch<A(!new)>(
+    m: map<var_name, var_name>, 
+    varDecls: seq<VarDecl>, 
+    varDecls': seq<VarDecl>,
+    p: Predicate<A>, 
+    q: Predicate<A>, 
+    s1: state<A>,
+    s2: state<A>,
+    s2Orig: MapOrig<Val<A>>)
+  requires RelPred(m, p, q, s2Orig)
+  requires 
+    && |varDecls| == |varDecls'|
+    && m.Values !! GetVarNames(varDecls')
+    && s2Orig.Keys !! GetVarNames(varDecls')
+    && RelState(m, s1, s2, s2Orig)
+  ensures 
+    var s2OrigNewKeys := set x | x in GetVarNames(varDecls) && x in m.Keys :: m[x];
+    var s2Orig' := s2Orig + map x' | x' in s2OrigNewKeys :: Maps.Get(s2, x');
+    var m' := m + ConvertVDeclsToSubstMap(varDecls, varDecls');
+    RelPred(m', ResetVarsPred(varDecls, p, s1), ResetVarsPred(varDecls', q, s2), s2Orig')
+  {
+    var s2OrigNewKeys := set x | x in GetVarNames(varDecls) && x in m.Keys :: m[x];
+    var s2Orig' := s2Orig + map x' | x' in s2OrigNewKeys :: Maps.Get(s2, x');
+    var m' := m + ConvertVDeclsToSubstMap(varDecls, varDecls');
+
+    forall sA, sB : state<A> | RelState(m', sA, sB, s2Orig')
+    ensures ResetVarsPred(varDecls, p, s1)(sA) == ResetVarsPred(varDecls', q, s2)(sB)
+    {
+      var sA' := ResetVarsState(varDecls, sA, s1);
+      var sB' := ResetVarsState(varDecls', sB, s2);
+
+      assert p(sA') == q(sB') by {
+        assert RelState(m, sA', sB', s2Orig) by {
+          RelStateSwitch(m, varDecls, varDecls', sA, sB, s1, s2, s2Orig);
+        }
+        reveal RelPred();
+      }
+    }
+
+    reveal RelPred();
+  }
+
+  lemma RelPostSwitch<A(!new)>(
+    m: map<var_name, var_name>, 
+    varDecls: seq<VarDecl>, 
+    varDecls': seq<VarDecl>,
+    post1: WpPostShallow<A>, 
+    post2: WpPostShallow<A>, 
+    s1: state<A>,
+    s2: state<A>,
+    s2Orig: MapOrig<Val<A>>)
+  requires RelPost(m, post1, post2, s2Orig)
+  requires 
+    && |varDecls| == |varDecls'|
+    && m.Values !! GetVarNames(varDecls')
+    && s2Orig.Keys !! GetVarNames(varDecls')
+    && RelState(m, s1, s2, s2Orig)
+  ensures 
+    var s2OrigNewKeys := set x | x in GetVarNames(varDecls) && x in m.Keys :: m[x];
+    var s2Orig' := s2Orig + map x' | x' in s2OrigNewKeys :: Maps.Get(s2, x');
+    var m' := m + ConvertVDeclsToSubstMap(varDecls, varDecls');
+    RelPost(m', ResetVarsPost(varDecls, post1, s1), ResetVarsPost(varDecls', post2, s2), s2Orig')
+  {
+    reveal RelPost();
+
+    var s2OrigNewKeys := set x | x in GetVarNames(varDecls) && x in m.Keys :: m[x];
+    var s2Orig' := s2Orig + map x' | x' in s2OrigNewKeys :: Maps.Get(s2, x');
+    var m' := m + ConvertVDeclsToSubstMap(varDecls, varDecls');
+
+    RelPredSwitch(m, varDecls, varDecls', post1.normal, post2.normal, s1, s2, s2Orig);
+    RelPredSwitch(m, varDecls, varDecls', post1.currentScope, post2.currentScope, s1, s2, s2Orig);
+    forall lbl | lbl in post1.scopes.Keys
+    ensures RelPred(m', ResetVarsPred(varDecls, post1.scopes[lbl], s1), ResetVarsPred(varDecls', post2.scopes[lbl], s2), s2Orig')
+    {
+      RelPredSwitch(m, varDecls, varDecls', post1.scopes[lbl], post2.scopes[lbl], s1, s2, s2Orig);
+    }
+  }
+
+  lemma ConvertVDeclsToSubstMapInj(varDecls: seq<VarDecl>, varDecls': seq<VarDecl>)
+  requires Sequences.HasNoDuplicates(GetVarNamesSeq(varDecls'))
+  requires |varDecls| == |varDecls'|
+  ensures 
+    && var res := ConvertVDeclsToSubstMap(varDecls, varDecls');
+    && Maps.Injective(res)
+  {
+    reveal Maps.Injective();
+
+    if |varDecls| > 0 {
+      var oldName:=  varDecls[0].0;
+      var newName := varDecls'[0].0;
+
+      var m' := ConvertVDeclsToSubstMap(varDecls[1..], varDecls'[1..]);
+
+      assert GetVarNamesSeq(varDecls'[1..]) == GetVarNamesSeq(varDecls')[1..];
+
+      assert Maps.Injective(m') by {
+        assert Sequences.HasNoDuplicates(GetVarNamesSeq(varDecls'[1..])) by {
+          reveal Sequences.HasNoDuplicates();
+        }
+
+        ConvertVDeclsToSubstMapInj(varDecls[1..], varDecls'[1..]);
+      }
+
+      var m := m'[oldName := newName];
+
+      forall x, x' | x != x' && x in m && x' in m 
+      ensures m[x] != m[x']
+      {
+        if x == oldName || x' == oldName {
+          var y' := if x == oldName then x' else x;
+
+          assert newName != m[y'] by {
+            assert m[y'] == m'[y'];
+            assert m'[y'] in GetVarNamesSeq(varDecls'[1..]) by {
+              assert m'[y'] in GetVarNames(varDecls'[1..]);
+              GetVarNamesContainedSeq(m'[y'], varDecls'[1..]);
+            }
+
+            /* 
+              Find two different indices in varDecls' that map to newName and m'[y'].
+              The lookups of those indices in varDecls' will trigger the Sequences.HasNoDuplicates
+              quantifier to then obtain the desired inequality. */
+
+            var j :| 1 <= j < |varDecls'| && GetVarNamesSeq(varDecls')[j] == m'[y'];
+
+            assert GetVarNamesSeq(varDecls')[0] == newName;
+            reveal Sequences.HasNoDuplicates();
+          }
+        } 
+      }
+    }
+  }
+
+  lemma StateUpdVarDeclsLookupAux<A>(s1: state<A>, s2: state<A>, varDecls: seq<(var_name, Ty)>, varDecls': seq<(var_name, Ty)>,vs: seq<Val<A>>, k: var_name)
+  requires |varDecls| == |varDecls'| == |vs|
+  requires k in GetVarNames(varDecls)
+  requires Sequences.HasNoDuplicates(GetVarNamesSeq(varDecls'))
+  ensures 
+    var m := ConvertVDeclsToSubstMap(varDecls, varDecls');
+    var s1' := StateUpdVarDecls(s1, varDecls, vs);
+    var s2' := StateUpdVarDecls(s2, varDecls', vs);
+    s1'[k] == s2'[m[k]]
+  { 
+    if |varDecls| == 0 {
+
+    } else {
+      var oldName := varDecls[0].0;
+      var newName := varDecls'[0].0;
+
+      var s1'' := StateUpdVarDecls(s1, varDecls[1..], vs[1..]);
+      var s2'' := StateUpdVarDecls(s2, varDecls'[1..], vs[1..]);
+
+      var s1' := s1''[oldName := vs[0]];
+      var s2' := s2''[newName := vs[0]];
+
+      var m'' := ConvertVDeclsToSubstMap(varDecls[1..], varDecls'[1..]);
+      var m' := m''[oldName := newName];
+
+      if k == oldName {
+
+      } else {
+        reveal Sequences.HasNoDuplicates();
+        assert m'[k] in GetVarNames(varDecls'[1..]);
+        assert GetVarNamesSeq(varDecls'[1..]) == GetVarNamesSeq(varDecls')[1..];
+        StateUpdVarDeclsLookupAux(s1, s2, varDecls[1..], varDecls'[1..], vs[1..], k);
+        assert m''[k] in GetVarNames(varDecls'[1..]);
+        assert m''[k] in GetVarNamesSeq(varDecls'[1..]) by {
+          GetVarNamesContainedSeq(m''[k], varDecls'[1..]);
+        }
+        assert m'[k] != newName by {
+          assert newName == GetVarNamesSeq(varDecls')[0];
+        }
+        calc {
+          s1'[k];
+          s1''[k];
+          s2''[m''[k]];
+          s2''[m'[k]];
+          s2'[m'[k]];
+        }
+      }
+    }
+  }
+
+  lemma ForallVarDeclsRelSwitch<A(!new)>(
+      a: absval_interp<A>, 
+      varDecls: seq<(var_name, Ty)>, 
+      varDecls': seq<(var_name, Ty)>,
+      m: map<var_name, var_name>, 
+      p1: Predicate<A>,
+      p2: Predicate<A>,
+      s1: state<A>,
+      s2: state<A>,
+      s2Orig: MapOrig<Val<A>>)
+      requires 
+        && |varDecls| == |varDecls'|
+        && (forall i | 0 <= i < |varDecls| :: varDecls[i].1 == varDecls'[i].1)
+      requires 
+        var s2OrigNewKeys := set x | x in GetVarNames(varDecls) && x in m.Keys :: m[x];
+        var s2Orig' := s2Orig + map x' | x' in s2OrigNewKeys :: Maps.Get(s2, x');
+        var m' := m + ConvertVDeclsToSubstMap(varDecls, varDecls');
+        && m.Values !! GetVarNames(varDecls')
+        && Sequences.HasNoDuplicates(GetVarNamesSeq(varDecls'))
+        && RelPred(m', p1, p2, s2Orig')
+        && RelState(m, s1, s2, s2Orig)
+        && s2Orig.Keys !! GetVarNames(varDecls')
+        //&& m'.Values !! s2Orig'.Keys
+      requires Maps.Injective(m)
+      ensures 
+        ForallVarDeclsShallow(a, varDecls, p1)(s1) == 
+        ForallVarDeclsShallow(a, varDecls', p2)(s2)
+  {
+    var s2OrigNewKeys := set x | x in GetVarNames(varDecls) && x in m.Keys :: m[x];
+    var s2Orig' := s2Orig + map x' | x' in s2OrigNewKeys :: Maps.Get(s2, x');
+    var m' := m + ConvertVDeclsToSubstMap(varDecls, varDecls');
+
+    forall vs | ValuesRespectDecls(a, vs, varDecls)
+    ensures p1(StateUpdVarDecls(s1, varDecls, vs)) == p2(StateUpdVarDecls(s2, varDecls', vs))
+    {
+      var s1' := StateUpdVarDecls(s1, varDecls, vs);
+      var s2' := StateUpdVarDecls(s2, varDecls', vs);
+      assert RelState(m', s1', s2', s2Orig') by {
+        reveal RelState();
+        forall k | k in m'.Keys 
+        ensures Maps.Get(s1', k) == Maps.Get(s2', m'[k])
+        {
+          if k in GetVarNames(varDecls) {
+            StateUpdVarDeclsLookupAux(s1, s2, varDecls, varDecls', vs, k);
+          } else {
+            assert m[k] == m'[k];
+            calc {
+              Maps.Get(s1', k);
+              { StateUpdVarDeclsLookup1(s1, varDecls, vs, k); }
+              Maps.Get(s1, k);
+              Maps.Get(s2, m[k]);
+              {
+                assert m[k] !in GetVarNames(varDecls');
+                StateUpdVarDeclsLookup1(s2, varDecls', vs, m[k]);
+              }
+              Maps.Get(s2', m'[k]);
+            }
+          }
+        }
+
+        forall k | k in s2Orig'.Keys
+        ensures Maps.Get(s2', k) == s2Orig'[k]
+        {
+          reveal RelState();
+          assert k !in GetVarNames(varDecls');
+          calc {
+            Maps.Get(s2', k);
+            { StateUpdVarDeclsLookup1(s2, varDecls', vs, k); }
+            Maps.Get(s2, k);
+          }
+        }
+        
+        assert m'.Values !! s2Orig'.Keys by {
+          assert m.Values !! s2Orig.Keys by {
+            reveal RelState();
+          }
+          assert m'.Values <= m.Values + GetVarNames(varDecls');
+
+          assert s2Orig'.Keys <= s2Orig.Keys + s2OrigNewKeys;
+
+          assert s2OrigNewKeys !! m'.Values by {
+            forall a, b | a in s2OrigNewKeys && b in m'.Values 
+            ensures a != b
+            {
+              var x :| x in GetVarNames(varDecls) && x in m.Keys && m[x] == a;
+              assert x in m.Keys;
+              assert m[x] == a;
+
+              assert m'[x] != m[x];
+
+              var y :| y in m'.Keys && m'[y] == b;
+
+              if y !in GetVarNames(varDecls) {
+                assert x != y;
+                calc {
+                  m'[y];
+                  m[y];
+                != { reveal Maps.Injective(); }
+                  m[x];
+                }
+              } else {
+                assert m'[y] in GetVarNames(varDecls');
+                assert m.Values !! GetVarNames(varDecls');
+              }
+            }
+          }
+        }
+      }
+      reveal RelPred();
+    }
+
+    ForallVarDeclsShallowEquiv(a, varDecls, varDecls', p1, p2, s1, s2);
+  } 
+
+  /** 
+   The lemma shows that if two postconditions post1 and post2 behave the same  
+   for states related via substMap (the mapping between active original variables
+   and their desugared counterparts), then the corresponding weakest preconditions
+   of the original and desugared programs must behave the same on related states.
+
+   The parameter s2Orig plays a key role in the proof of scopes.  Suppose 
+
+    Scope {
+      var x: int
+      ...
+      Scope {
+        var x: int
+        ...
+      }
+    } 
+    
+    is desugared to
+    
+    Scope {
+      var x1: int
+      ...
+      Scope {
+        var x2: int
+        ...
+      }
+    } 
+
+  When proving the relationship between outer scopes, in the proof, s2Orig is chosen to be
+  the empty map.
+  When proving the relationship between the inner scopes, s2Orig is chosen to be 
+  the singleton map where x1 maps to the value that x1 had right before executing the inner scope.
+  In general, the domain of s2Orig is the set of desugared variables that are currently shadowed.
+
+  RelState(..., ..., s2, s2Orig) ensures that the state s2 in the desugared program coincides
+  with s2Orig on s2Orig's domain. That is, in the proof, it makes explicit that shadowed 
+  variables cannot be modified. This is essential in the scopes case, because if shadowed variables 
+  were modified, then one cannot prove that the programs after the scopes are related.
+  In terms of weakest preconditions, this means that we cannot use the fact that the 
+  given postconditions post1 and post2 are related, because this relationship holds only
+  if the shadowed variabels are not modified.  
+  */
+  lemma {:induction false} MakeScopedVarsUniqueCorrect<A(!new)>(
+        a: absval_interp<A>,
+        c: Cmd, 
+        substMap: map<var_name, var_name>, 
+        counter: nat,
+        post1: WpPostShallow<A>,
+        post2: WpPostShallow<A>,
+        s2Orig: MapOrig<Val<A>>,
+        names: set<string>)
+      requires c.WellFormedVars(substMap.Keys)
+      requires Maps.Injective(substMap)
+      requires 
+        var (c', counter') := MakeScopedVarsUnique(c, substMap, counter);
+        && LabelsWellDefAux(c, post1.scopes.Keys) 
+        && LabelsWellDefAux(c', post2.scopes.Keys)
+        && RelPost(substMap, post1, post2, s2Orig)
+        && s2Orig.Keys <= VarNameSet(names, 0, counter)
+        && substMap.Values <= VarNameSet(names, 0, counter) 
+      //requires forall vDecl | vDecls in seqSubstMap :: substMap(vDecl.) == sequSubstMap
+      ensures 
+        var (c', counter') := MakeScopedVarsUnique(c, substMap, counter);
+        RelPred(substMap, WpShallow(a, c, post1), WpShallow(a, c', post2), s2Orig)
+    {
+      reveal RelPost();
+      match c {
+        case SimpleCmd(sc) =>
+          reveal WpShallow();
+          SubstSimpleCmdCorrect(a, sc, substMap, post1.normal, post2.normal, s2Orig);
+        case Break(_) => reveal WpShallow();
+        case Seq(c1, c2) => 
+          var (c1', counter1') := MakeScopedVarsUnique(c1, substMap, counter);
+          var (c2', counter2') := MakeScopedVarsUnique(c2, substMap, counter1');
+
+          var post1' := WpPostShallow(WpShallow(a, c2, post1), post1.currentScope, post1.scopes);
+          var post2' := WpPostShallow(WpShallow(a, c2', post2), post2.currentScope, post2.scopes);
+
+          assert RelPost(substMap, post1', post2', s2Orig) by {
+            assert RelPred(substMap, WpShallow(a, c2, post1), WpShallow(a, c2', post2), s2Orig) by {
+              VarNameSetExtend(names, 0, counter, counter1');
+              MakeScopedVarsUniqueCorrect(a, c2, substMap, counter1', post1, post2, s2Orig, names);
+            }
+          }
+
+          assert RelPred(substMap, WpShallow(a, c1, post1'), WpShallow(a, c1', post2'), s2Orig) by {
+            MakeScopedVarsUniqueCorrect(a, c1, substMap, counter, post1', post2', s2Orig, names);
+          }
+
+          reveal WpShallow();
+        case Scope(optLabel, varDecls, body) => 
+          /* Goal: RelPred(substMap, WpShallow(a, c, post1), WpShallow(a, c', post2)) */
+          var varDecls' := CreateUniqueVarDecls(varDecls, counter);
+
+          assert Sequences.HasNoDuplicates(GetVarNamesSeq(varDecls')) by {
+            CreateUniqueVarDeclsNoDup(varDecls, counter);
+          }
+
+          var counter' := counter + |varDecls'|;
+          var substMap' := substMap + ConvertVDeclsToSubstMap(varDecls, varDecls');
+          assert substMap'.Keys == GetVarNames(varDecls)+substMap.Keys;
+          var (body', counter'') := MakeScopedVarsUnique(body, substMap', counter');
+          //(Scope(optLabel, varDecls', body''), counter'')
+          var c' := Scope(optLabel, varDecls', body');
+
+          var updatedScopes1 := 
+            if optLabel.Some? then 
+              post1.scopes[optLabel.value := post1.normal]
+            else post1.scopes;
+          assert updatedScopes1.Keys == if optLabel.Some? then {optLabel.value} + post1.scopes.Keys else post1.scopes.Keys;
+          
+          var updatedScopes2 := 
+            if optLabel.Some? then 
+              post2.scopes[optLabel.value := post2.normal]
+            else post2.scopes;
+          assert updatedScopes2.Keys == if optLabel.Some? then {optLabel.value} + post2.scopes.Keys else post2.scopes.Keys;
+          
+          var post1' := WpPostShallow(post1.normal, post1.normal, updatedScopes1);
+          var post2' := WpPostShallow(post2.normal, post2.normal, updatedScopes2);
+
+          forall s1,s2 | RelState(substMap, s1, s2, s2Orig)
+          ensures WpShallow(a, c, post1)(s1) == WpShallow(a, c', post2)(s2)
+          {
+            /* We want to prove that if a name x in varDecls is already mapped to x' in substMap, then 
+              it must be the case that x' will not be modified within the scope, since we map x to a new
+              name and x' won't be reused in the scope. We need this to make sure that when the scope is finished
+              and the variables are reset, x and x' are again related in the resulting states (
+                for x we know the value is reset to the previous value, for x' we prove the value cannot have changed
+              ). */
+            var s2OrigNewKeys := set x | x in GetVarNames(varDecls) && x in substMap.Keys :: substMap[x];
+            var s2Orig' := s2Orig + map x' | x' in s2OrigNewKeys :: Maps.Get(s2, x');
+
+            assert 
+              && substMap.Values !! GetVarNames(varDecls')
+              && s2Orig.Keys !! GetVarNames(varDecls') by {
+              VarNameSetDisjoint(names, GetVarNames(varDecls), 0, counter, counter, counter + |varDecls'|);
+            }
+
+            calc {
+              WpShallow(a, Scope(optLabel, varDecls, body), post1)(s1);
+              {reveal WpShallow();}
+              ForallVarDeclsShallow(a, varDecls, WpShallow(a, body, ResetVarsPost(varDecls, post1', s1)))(s1);
+              { 
+                assert RelPost(substMap', ResetVarsPost(varDecls, post1', s1), ResetVarsPost(varDecls', post2', s2), s2Orig') by 
+                { 
+                  assert RelPost(substMap, post1, post2, s2Orig);
+
+                  assert RelPost(substMap, post1', post2', s2Orig);
+                  {
+                    reveal RelPost();
+                  }
+
+                  RelPostSwitch(substMap, varDecls, varDecls', post1', post2', s1, s2, s2Orig);
+                }
+
+                assert Maps.Injective(substMap') by {
+                  assert Maps.Injective(ConvertVDeclsToSubstMap(varDecls, varDecls')) by {
+                    ConvertVDeclsToSubstMapInj(varDecls, varDecls');
+                  }
+                  assert substMap.Values !! GetVarNames(varDecls');
+                  UnionOfInjectiveMaps(substMap, ConvertVDeclsToSubstMap(varDecls, varDecls'));
+                }
+
+                assert RelPred(substMap', 
+                  WpShallow(a, body, ResetVarsPost(varDecls, post1', s1)), 
+                  WpShallow(a, body', ResetVarsPost(varDecls', post2', s2)),
+                  s2Orig') by
+                  { 
+                    assert s2Orig'.Keys <= VarNameSet(names+GetVarNames(varDecls), 0, counter') by {
+                      VarNameSetExtend2(names, GetVarNames(varDecls), 0, counter, counter');
+                    }
+
+                    assert substMap'.Values <= VarNameSet(names+GetVarNames(varDecls), 0, counter') by {
+                      assert substMap'.Values <= VarNameSet(names, 0, counter) + VarNameSet(GetVarNames(varDecls), counter, counter + |varDecls|);
+                      VarNameSetAppend(names, GetVarNames(varDecls), 0, counter, counter, counter + |varDecls|);
+                    }
+
+                    MakeScopedVarsUniqueCorrect(
+                      a, body, substMap', counter',  ResetVarsPost(varDecls, post1', s1), ResetVarsPost(varDecls', post2', s2), s2Orig',
+                      names+GetVarNames(varDecls)
+                    ); 
+                  }
+                  
+                  var p1 := WpShallow(a, body, ResetVarsPost(varDecls, post1', s1));
+                  var p2 := WpShallow(a, body', ResetVarsPost(varDecls', post2', s2));
+
+                  ForallVarDeclsRelSwitch(
+                      a, 
+                      varDecls, 
+                      varDecls',
+                      substMap, 
+                      p1,
+                      p2,
+                      s1,
+                      s2,
+                      s2Orig);
+              }
+              ForallVarDeclsShallow(a, varDecls', WpShallow(a, body', ResetVarsPost(varDecls', post2', s2)))(s2);
+              {reveal WpShallow();}
+              WpShallow(a, Scope(optLabel, varDecls', body'), post2)(s2);
+            }
+          }
+
+          reveal RelPred();
+        case If(None, thn, els) => 
+          var (thn', counter') := MakeScopedVarsUnique(thn, substMap, counter);
+          var (els', counter'') := MakeScopedVarsUnique(els, substMap, counter');
+
+          assert RelPred(substMap, WpShallow(a, thn, post1), WpShallow(a, thn', post2), s2Orig) by {
+            MakeScopedVarsUniqueCorrect(a, thn, substMap, counter, post1, post2, s2Orig, names);
+          }
+
+          assert RelPred(substMap, WpShallow(a, els, post1), WpShallow(a, els', post2), s2Orig) by {
+            VarNameSetExtend(names, 0, counter, counter');
+            MakeScopedVarsUniqueCorrect(a, els, substMap, counter', post1, post2, s2Orig, names);
+          }
+
+          reveal RelPred();
+
+          forall sA, sB | RelState(substMap, sA, sB, s2Orig)
+          ensures WpShallow(a, c, post1)(sA) == WpShallow(a, If(None, thn', els'), post2)(sB)
+          {
+            calc {
+              WpShallow(a, c, post1)(sA);
+              { reveal WpShallow(); }
+              Util.AndOpt(WpShallow(a, thn, post1)(sA), WpShallow(a, els, post1)(sA));
+              Util.AndOpt(WpShallow(a, thn', post2)(sB), WpShallow(a, els', post2)(sB));
+              { reveal WpShallow(); }
+              WpShallow(a, If(None, thn', els'), post2)(sB);
+            }
+          }
+        case _ => assume false;
+      }
+    }
+
+}
